Locality.thy
@@ -1,337 +1,366 @@
 theory Locality
-  imports "Algebra/PartialMonoid" While
+  imports "Algebra/PartialMonoid"
 begin
 
+text {*
+  We define a separation algebra on a set of pair, where the first
+  component contains no algebraic structure and the second is
+  a partial commutative monoid.
+*}
+
+text {* Notation *}
+
 no_notation times (infixl "*" 70)
-
-type_synonym heap = "nat \<Rightarrow> nat option"
-
-definition ortho :: "heap \<Rightarrow> heap \<Rightarrow> bool" (infix "\<bottom>" 55)
-  where "h1 \<bottom> h2 \<equiv> dom h1 \<inter> dom h2 = {}"
+  and pmult_defined (infix "##" 55)
 
 (*********************************************************************************************)
 
-text {* State Level *}
-
-type_synonym 's state = "('s \<times> heap) option"
-
-abbreviation fault_state :: "'s state" ("fault") where "fault \<equiv> None"
-abbreviation some_state :: "'s \<Rightarrow> heap \<Rightarrow> 's state" ("<_, _>") where "<s, h> \<equiv> Some (s, h)"
-
-definition state_def :: "'s state \<Rightarrow> 's state \<Rightarrow> bool" (infix "##" 50) where
-  "\<sigma> ## \<sigma>' \<equiv> case \<sigma> of fault \<Rightarrow> False
-                     | <s, h> \<Rightarrow> (case \<sigma>' of fault \<Rightarrow> False
-                                          | <s', h'> \<Rightarrow> s = s' \<and> h \<bottom> h')"
-
-definition state_sep :: "'s state \<Rightarrow> 's state \<Rightarrow> 's state" (infixl "\<bullet>" 70) where
-  "\<sigma> \<bullet> \<sigma>' \<equiv> case \<sigma> of fault \<Rightarrow> fault
-                    | <s, h> \<Rightarrow> (case \<sigma>' of fault \<Rightarrow> fault
-                                         | <s', h'> \<Rightarrow> (if s = s' \<and> h \<bottom> h' then <s, h ++ h'> else fault))"
-
-definition state_leq :: "'s state \<Rightarrow> 's state \<Rightarrow> bool" (infix "\<preceq>" 50) where
-  "\<sigma> \<preceq> \<sigma>' \<equiv> \<exists>\<delta>. \<sigma> ## \<delta> \<and> \<sigma>' = \<sigma> \<bullet> \<delta>"
-
-interpretation state: partial_ab_semigroup state_sep state_def
-  apply default
-  apply (auto simp: state_def_def state_sep_def)
-    apply (case_tac x, auto)
-    apply (case_tac y, auto)
-    apply (case_tac z, auto simp: ortho_def)
-  apply auto
-    apply (case_tac x, auto)
-    apply (case_tac y, force)
-    apply (case_tac z, auto simp: ortho_def)
-  apply auto
-    apply (case_tac x, auto)
-    apply (case_tac y, auto)
-    apply (case_tac z, auto)
-  apply (auto simp: ortho_def)
-    apply (case_tac x, auto)
-  apply (case_tac y, auto simp: ortho_def)
-    apply (case_tac x, auto)
-    apply (case_tac y, auto simp: ortho_def map_add_comm)
-  apply auto
-done
-
-lemma state_leq_sep1: "\<sigma> ## \<sigma>' \<Longrightarrow> \<sigma> \<preceq> \<sigma> \<bullet> \<sigma>'"
-  by (auto simp add: state_sep_def state_def_def state_leq_def)
-
-lemma state_leq_sep2: "\<sigma> ## \<sigma>' \<Longrightarrow> \<sigma>' \<preceq> \<sigma> \<bullet> \<sigma>'"
-  using state.pmult_comm state.pmult_comm_def state_leq_def by blast
-
-lemma state_leq_fault1 [simp]: "\<not> fault \<preceq> \<sigma>"
-  by (auto simp: state_leq_def state_def_def)
-
-lemma state_leq_fault2 [simp]: "\<not> \<sigma> \<preceq> fault"
-  by (auto simp: state_leq_def state_def_def state_sep_def split: option.split)
-
-lemma state_defD [dest]: "\<sigma> ## \<sigma>' \<Longrightarrow> \<exists>s h h'. \<sigma> = Some (s, h) \<and> \<sigma>' = Some (s, h') \<and> h \<bottom> h'"
-  apply (auto simp: state_def_def)
-  apply (cases \<sigma>)
-  apply auto
-  apply (cases \<sigma>')
-  apply auto
-done
-
-lemma state_non_fault1 [simp]: "\<sigma> ## \<sigma>' \<Longrightarrow> \<sigma> \<noteq> fault"
-  by auto
-
-lemma state_non_fault2 [simp]: "\<sigma> ## \<sigma>' \<Longrightarrow> \<sigma>' \<noteq> fault"
-  by auto
-
-lemma state_sep_non_fault1 [simp]: "\<sigma> ## \<sigma>' \<Longrightarrow> \<sigma> \<bullet> \<sigma>' \<noteq> fault"
-  by (auto simp: state_sep_def)
-
-lemma state_sep_non_fault2 [simp]: "\<sigma> ## \<sigma>' \<Longrightarrow> \<sigma>' \<bullet> \<sigma> \<noteq> fault"
-  using state.pmult_comm_def state_sep_non_fault1 by blast
-
-lemma state_sep_unfold: "<s, h> = \<delta> \<bullet> <s', h'> \<Longrightarrow> \<exists>dh. h = dh ++ h' \<and> dh \<bottom> h' \<and> s = s' \<and> \<delta> = <s, dh>"
-  apply (auto simp: state_sep_def)
-  apply (cases \<delta>)
-  -- None apply clarsimp
-  -- Some 
-    apply clarsimp 
-    apply (case_tac "a = s' \<and> b \<bottom> h'")
-    apply auto
-done
-
-(*********************************************************************************************)
-
-text {* Predicate (Assertion) Level *}
-
-type_synonym 's pred = "('s \<times> heap) set option"
-
-abbreviation fault_pred :: "'s pred" ("Fault") where "Fault \<equiv> None"
+abbreviation univ_pred :: "'a set" ("\<top>") where "\<top> \<equiv> UNIV"
+abbreviation fault_pred :: "'a set option" ("\<bottom>") where "\<bottom> \<equiv> None"
 abbreviation some_pred :: "'a \<Rightarrow> 'a option" ("<_>") where "<P> \<equiv> Some P"
-                               
 
-definition sep_conj :: "'s pred \<Rightarrow> 's pred \<Rightarrow> 's pred" (infixl "*" 75) where
-  "P * Q \<equiv> case P of Fault \<Rightarrow> None 
-                | <p> \<Rightarrow> (case Q of Fault \<Rightarrow> Fault 
-                               | <q> \<Rightarrow> <{(s, h ++ h') | s s' h h' . s = s' \<and> h \<bottom> h' \<and> (s, h) \<in> p \<and> (s', h') \<in> q}>)"
+type_synonym ('a, 'b) state = "('a \<times> 'b) option"
+type_synonym ('a, 'b) pred = "('a \<times> 'b) set"
+type_synonym ('a, 'b) pred_bot = "('a \<times> 'b) set option"
+type_synonym 'b hpred = "'b set"
+type_synonym 'b hpred_bot = "'b set option"
 
-definition emp :: "'s pred" where "emp \<equiv> <{(s, h) | s h. h = Map.empty}>"
+abbreviation fault_state :: "('a, 'b) state" ("fault") where "fault \<equiv> None"
+abbreviation some_state :: "'a \<Rightarrow> 'b \<Rightarrow> ('a, 'b) state" ("<_, _>") where "<s, h> \<equiv> Some (s, h)"
 
-definition pred_leq :: "'s pred \<Rightarrow> 's pred \<Rightarrow> bool" (infixl "\<sqsubseteq>" 50) where
-  "P \<sqsubseteq> Q \<equiv> case P of Fault \<Rightarrow> Q = Fault
-                    | <p> \<Rightarrow> (case Q of Fault \<Rightarrow> True
-                                     | <q> \<Rightarrow> p \<le> q)"
+(*********************************************************************************************)
 
-definition pred_le :: "'s pred \<Rightarrow> 's pred \<Rightarrow> bool" (infixl "\<sqsubset>" 50) where
-  "P \<sqsubset> Q \<equiv> P \<sqsubseteq> Q \<and> P \<noteq> Q"
+text {* Locality is defined on the abstract concept of separation algebra *}
 
-interpretation pred: monoid sep_conj emp
-  apply default
-  apply (auto simp: sep_conj_def emp_def)
-    apply (case_tac a, auto)
-    apply (case_tac b, auto)
-    apply (case_tac c, auto simp: ortho_def)
-    apply (metis (no_types, lifting) Un_empty dom_map_add inf_sup_distrib1 inf_sup_distrib2 map_add_assoc)
-  apply (metis (no_types, lifting) Un_empty dom_map_add inf_sup_distrib1 inf_sup_distrib2 map_add_assoc)
-  apply (case_tac a, auto simp: ortho_def)
-  apply (case_tac a, auto simp: ortho_def)
-done
+locale locality  = partial_comm_monoid sep_add sep_def sep_unit
+  for sep_add :: "'b \<Rightarrow> 'b \<Rightarrow> 'b" (infixl "\<bullet>" 70)
+    and sep_def :: "'b \<Rightarrow> 'b \<Rightarrow> bool" (infix "##" 50)
+    and sep_unit :: 'b ("emp")
+begin
 
-lemma Fault_annir [simp]: "P * Fault = Fault"
-  apply (auto simp: sep_conj_def)
-  apply (cases P)
-  apply auto
-done
+text {* Sub state relation *}
 
-lemma Fault_annil [simp]: "Fault * P = Fault"
-  by (auto simp: sep_conj_def)
+definition substate :: "'b \<Rightarrow> 'b \<Rightarrow> bool" (infix "\<preceq>" 50) where
+  "x \<preceq> y \<equiv> \<exists>z. x ## z \<and> y = x \<bullet> z"
 
-lemma FaultI1:"P * <q> = Fault \<Longrightarrow> P = Fault"
-  apply (clarsimp simp: sep_conj_def)
+lemma substate_trans: "x \<preceq> y \<Longrightarrow> y \<preceq> z \<Longrightarrow> x \<preceq> z"
+  using local.pmult_ab1 local.pmult_assoc substate_def by fastforce
+
+text {* Predicate about the heap *}
+
+definition sep_hset :: "'b hpred \<Rightarrow> 'b hpred \<Rightarrow> 'b hpred" (infixl "*\<^sup>h" 75) where
+  "P *\<^sup>h Q = { h \<bullet> h' | h h' . h ## h' \<and> h \<in> P \<and> h' \<in> Q}"
+
+fun sepbot_hset :: "'b hpred_bot \<Rightarrow> 'b hpred_bot \<Rightarrow> 'b hpred_bot" (infixl "*\<^sup>h\<^sub>\<bottom>" 75) where
+  "<P> *\<^sup>h\<^sub>\<bottom> <Q> = <{ h \<bullet> h' | h h' . h ## h' \<and> h \<in> P \<and> h' \<in> Q}>"
+| "p *\<^sup>h\<^sub>\<bottom> \<bottom> = \<bottom>"
+| "\<bottom> *\<^sup>h\<^sub>\<bottom> q = \<bottom>"
+
+definition EMPH :: "'b hpred_bot" where "EMPH \<equiv> <{emp}>"
+
+fun leq_hset :: "'b hpred_bot \<Rightarrow> 'b hpred_bot \<Rightarrow> bool" (infixl "\<subseteq>\<^sup>h\<^sub>\<bottom>" 50) where
+  "<P> \<subseteq>\<^sup>h\<^sub>\<bottom> <Q> \<longleftrightarrow> P \<subseteq> Q"
+| "p \<subseteq>\<^sup>h\<^sub>\<bottom> \<bottom> \<longleftrightarrow> True"
+| "\<bottom> \<subseteq>\<^sup>h\<^sub>\<bottom> q \<longleftrightarrow> q = \<bottom>"
+
+definition le_hset :: "'b hpred_bot \<Rightarrow> 'b hpred_bot \<Rightarrow> bool" (infixl "\<subset>\<^sup>h\<^sub>\<bottom>" 50) where
+  "P \<subset>\<^sup>h\<^sub>\<bottom> Q \<equiv> P \<subseteq>\<^sup>h\<^sub>\<bottom> Q \<and> P \<noteq> Q"
+
+(* TODO: interpret sep_hset as a quantale *)
+
+lemma sepbot_hset_botl [simp]: "\<bottom> *\<^sup>h\<^sub>\<bottom> Q = \<bottom>"
+  using sepbot_hset.elims by auto
+
+lemma sepbot_hset_eqbot [iff]:"P *\<^sup>h\<^sub>\<bottom> <Q> = \<bottom> \<longleftrightarrow> P = \<bottom>"
   by (cases P) auto
 
-lemma FaultI2:"<p> * Q = Fault \<Longrightarrow> Q = Fault"
-  apply (clarsimp simp: sep_conj_def)
+lemma leq_hset_refl [intro]: "P \<subseteq>\<^sup>h\<^sub>\<bottom> P"
+  by (cases P) auto
+
+lemma leq_hset_eqbot [simp]: "\<bottom> \<subseteq>\<^sup>h\<^sub>\<bottom> Q \<longleftrightarrow> Q = \<bottom>"
   by (cases Q) auto
 
-interpretation order pred_leq pred_le
-  apply default
-  apply (auto simp: pred_leq_def pred_le_def)
-    apply (case_tac x, auto)
-  apply (case_tac y, auto)
-  apply (case_tac x, auto)
-    apply (case_tac x, auto)
-    apply (case_tac y, auto)
-  apply (case_tac z, auto)
-    apply (case_tac x, auto)
-  apply (case_tac y, auto)
-done
 
 (*********************************************************************************************)
 
 text {* Safety and Framing properties on Relations *}
 
-definition safe :: "'s state rel \<Rightarrow> bool" where
-  "safe R \<equiv> \<forall>\<sigma> \<sigma>'. (\<sigma>, None) \<notin> R \<and> \<sigma> \<preceq> \<sigma>' \<longrightarrow> (\<sigma>', None) \<notin> R"
+definition safe :: "('a, 'b) state rel \<Rightarrow> bool" where
+  "safe R \<equiv> \<forall>s h h'. (<s, h>, fault) \<notin> R \<and> h \<preceq> h' \<longrightarrow> (<s, h'>, fault) \<notin> R"
 
-definition frame :: "'s state rel \<Rightarrow> bool" where
-  "frame R \<equiv> \<forall>\<sigma>o \<sigma> \<sigma>1 \<sigma>'. (\<sigma>o, None) \<notin> R \<and> \<sigma>o ## \<sigma>1 \<and> \<sigma> = \<sigma>o \<bullet> \<sigma>1 \<and> (\<sigma>, \<sigma>') \<in> R \<longrightarrow> (\<exists>\<sigma>o'. \<sigma>' = \<sigma>o' \<bullet> \<sigma>1 \<and> (\<sigma>o, \<sigma>o') \<in> R)" 
-
-lemma safe_fault: "safe R \<Longrightarrow> (\<sigma>o, fault) \<notin> R \<Longrightarrow> \<sigma>o ## \<sigma>1 \<Longrightarrow> (\<sigma>o \<bullet> \<sigma>1, fault) \<notin> R"
-  using safe_def state_leq_sep1 by blast
+definition frame :: "('a, 'b) state rel \<Rightarrow> bool" where
+  "frame R \<equiv> \<forall>so ho h dh s' h'. 
+              (<so, ho>, fault) \<notin> R \<and>
+              ho ## dh \<and> 
+              h = ho \<bullet> dh \<and>                    
+              (<so, h>, <s', h'>) \<in> R
+              \<longrightarrow> (\<exists>so' ho'. ho' ## dh \<and> h' = ho' \<bullet> dh \<and> (<so, ho>, <so', ho'>) \<in> R)" 
 
 (*********************************************************************************************)
 
 text {* State Transformer *}
 
-definition func :: "'s state rel \<Rightarrow> 's state \<Rightarrow> 's pred" ("\<langle>_\<rangle>" [50] 1000) where
-  "func R \<sigma> \<equiv> case \<sigma> of fault \<Rightarrow> Fault | 
-                  <(s, h)> \<Rightarrow> (if (\<sigma>, fault) \<in> R then Fault 
-                                                else <{(s', h') | s' h'. (<s, h>, <s', h'>) \<in> R}>)"
+definition stran :: "('a, 'b) state rel \<Rightarrow> 'a \<Rightarrow> 'b \<Rightarrow> ('a, 'b) pred_bot" ("\<langle>_\<rangle>") where
+  "\<langle>R\<rangle> s h \<equiv> if (<s, h>, fault) \<in> R then \<bottom> else <{(s', h'). (<s, h>, <s', h'>) \<in> R}>"
 
-lemma func_faultD [dest]: "(\<sigma>, fault) \<in> R \<Longrightarrow> \<langle>R\<rangle> \<sigma> = Fault"
-  by (auto simp: func_def split: option.split)
+lemma non_fault_eq: "\<exists>P. \<langle>R\<rangle> s h = <P> \<longleftrightarrow> (<s, h>, fault) \<notin> R"
+  by (clarsimp simp: stran_def)
 
-lemma func_non_FaultD [dest]: "\<langle>R\<rangle> \<sigma> \<noteq> Fault \<Longrightarrow> (\<sigma>, fault) \<notin> R"
-  by (meson func_faultD)
+lemma non_faultD [dest]: "\<langle>R\<rangle> s h = <P> \<Longrightarrow> (<s, h>, fault) \<notin> R"
+  by (clarsimp simp: stran_def)
 
-lemma func_fault_eq [simp]: "\<sigma> \<noteq> fault \<Longrightarrow> \<langle>R\<rangle> \<sigma> = Fault \<longleftrightarrow> (\<sigma>, fault) \<in> R"
-  by (auto simp: func_def split: option.split)
+lemma fault_eq: "\<langle>R\<rangle> s h = \<bottom> \<longleftrightarrow> (<s, h>, fault) \<in> R"
+  by (auto simp: stran_def)
 
-lemma func_some: "\<langle>R\<rangle> \<sigma> = <S> \<Longrightarrow> \<sigma>' \<in> S \<Longrightarrow> (\<sigma>, <\<sigma>'>) \<in> R"
-  apply (auto simp: func_def)
-  apply (cases \<sigma>)
-  apply auto
-  apply (case_tac "(<a, b>, fault) \<in> R")
-  apply auto
-done
+lemma safeD1: "safe R \<Longrightarrow> (<s, h'>, fault) \<in> R \<Longrightarrow> h \<preceq> h' \<Longrightarrow> (<s, h>, fault) \<in> R"
+  using safe_def by fastforce
 
-lemma func_some2: "\<langle>R\<rangle> <s, h> = <S> \<Longrightarrow> (<s, h>, <s', h'>) \<in> R \<Longrightarrow> (s', h') \<in> S"
-  apply (auto simp: func_def)
+lemma safeD2: "safe R \<Longrightarrow> h ## h' \<Longrightarrow> \<langle>R\<rangle> s (h \<bullet> h') = \<bottom> \<Longrightarrow> \<langle>R\<rangle> s h = \<bottom>"
+  by (meson fault_eq substate_def safe_def)
+
+primrec image_bot :: "('c \<Rightarrow> 'd) \<Rightarrow> 'c set option \<Rightarrow> 'd set option" (infixr "``" 90) where
+  "f `` \<bottom> = \<bottom>"
+| "f `` <A> = <{y. \<exists>x\<in>A. y = f x}>"
+
+abbreviation hproj :: "('a, 'b) pred \<Rightarrow> 'b hpred" ("_\<downharpoonright>\<^sup>h" [1000] 999) where
+  "P\<downharpoonright>\<^sup>h \<equiv> snd ` P"
+
+lemma hprojI [intro]: "(s, h) \<in> P \<Longrightarrow>  h \<in> P\<downharpoonright>\<^sup>h"
+  by (simp add: rev_image_eqI)
+
+abbreviation hproj_bot :: "('a, 'b) pred_bot \<Rightarrow> 'b hpred_bot" ("_\<downharpoonright>\<^sup>h\<^sub>\<bottom>" [1000] 999) where
+  "P\<downharpoonright>\<^sup>h\<^sub>\<bottom> \<equiv> snd `` P"
+
+lemma hproj_bot: "f = \<bottom> \<Longrightarrow> (f)\<downharpoonright>\<^sup>h\<^sub>\<bottom> = \<bottom>"
+  by auto
+
+lemma hproj_some [simp]: "f = <P> \<Longrightarrow> (f)\<downharpoonright>\<^sup>h\<^sub>\<bottom> = <P\<downharpoonright>\<^sup>h >"
+  by auto
+
+lemma safeD2_hproj: "safe R \<Longrightarrow> h ## h' \<Longrightarrow> (\<langle>R\<rangle> s (h \<bullet> h'))\<downharpoonright>\<^sup>h\<^sub>\<bottom> = \<bottom> \<Longrightarrow> (\<langle>R\<rangle> s h)\<downharpoonright>\<^sup>h\<^sub>\<bottom> = \<bottom>"
+  by (metis (no_types, lifting) image_bot.simps(2) option.distinct(1) safeD2 stran_def)
+
+lemma non_faultD_hproj [dest]: "(\<langle>R\<rangle> s h)\<downharpoonright>\<^sup>h\<^sub>\<bottom> = <P> \<Longrightarrow> (<s, h>, fault) \<notin> R"
+  by (clarsimp simp: stran_def)
+
+lemma stran_hproj_eq: "(\<langle>R\<rangle> s h)\<downharpoonright>\<^sup>h\<^sub>\<bottom> = <H> \<Longrightarrow> h' \<in> H \<longleftrightarrow> (\<exists>s'. (<s, h>, <s', h'>) \<in> R)"
+  apply (clarsimp simp: stran_def)
   apply (case_tac "(<s, h>, fault) \<in> R")
   apply auto
 done
 
+lemma stran1: "(\<langle>R\<rangle> s h)\<downharpoonright>\<^sup>h\<^sub>\<bottom> = <H> \<Longrightarrow> \<exists>s' h'. h' \<in> H \<longrightarrow> (<s, h>, <s', h'>) \<in> R"
+  by (auto simp: stran_hproj_eq)
 
+lemma stran2: "(\<langle>R\<rangle> s h)\<downharpoonright>\<^sup>h\<^sub>\<bottom> = <H> \<Longrightarrow> h' \<in> H \<Longrightarrow> \<exists>s'. (<s, h>, <s', h'>) \<in> R"
+  by (auto simp: stran_hproj_eq)
 
-(*********************************************************************************************)
+lemma stran3: "(\<langle>R\<rangle> s h)\<downharpoonright>\<^sup>h\<^sub>\<bottom> = <H> \<Longrightarrow> (<s, h>, <s', h'>) \<in> R \<Longrightarrow> h' \<in> H"
+  by (auto simp: stran_hproj_eq)
 
 text {* Locality -- State Transformer *}
 
-definition local :: "('s state \<Rightarrow> 's pred) \<Rightarrow> bool" where
-  "local f \<equiv> \<forall>\<sigma> \<sigma>'. \<sigma> ## \<sigma>' \<longrightarrow> f (\<sigma> \<bullet> \<sigma>') \<sqsubseteq> (f \<sigma>) * <{the \<sigma>'}>"
+definition local :: "('a \<Rightarrow> 'b \<Rightarrow> ('a, 'b) pred_bot) \<Rightarrow> bool" where
+  "local f \<equiv> \<forall>s h h'. h ## h' \<longrightarrow> (f s (h \<bullet> h'))\<downharpoonright>\<^sup>h\<^sub>\<bottom> \<subseteq>\<^sup>h\<^sub>\<bottom> (f s h)\<downharpoonright>\<^sup>h\<^sub>\<bottom> *\<^sup>h\<^sub>\<bottom> <{h'}>"
 
-lemma frame_local_Fault: "safe R \<Longrightarrow> \<sigma> ## \<sigma>' \<Longrightarrow> \<langle>R\<rangle> (\<sigma> \<bullet> \<sigma>') = Fault \<Longrightarrow> \<langle>R\<rangle> \<sigma> * <{the \<sigma>'}> = Fault"
-  by clarsimp (metis Fault_annil func_non_FaultD safe_def state_leq_sep1)
-
-lemma frame_local_Some: "safe R \<Longrightarrow> frame R \<Longrightarrow> \<sigma> ## \<sigma>' \<Longrightarrow> \<langle>R\<rangle> (\<sigma> \<bullet> \<sigma>') = <P> \<Longrightarrow> \<langle>R\<rangle> \<sigma> * <{the \<sigma>'}> = <Q> \<Longrightarrow> P \<subseteq> Q"
-  apply (clarsimp simp: frame_def sep_conj_def)
-  apply (cases "\<langle>R\<rangle> \<sigma>")
-  -- None apply clarsimp
-  -- Some 
-    apply (frule state_defD)
+theorem sf_local: "safe R \<Longrightarrow> frame R \<Longrightarrow> local \<langle>R\<rangle>"
+  apply (clarsimp simp: local_def)
+  apply (case_tac "(\<langle>R\<rangle> s h)\<downharpoonright>\<^sup>h\<^sub>\<bottom>")
+  -- None
     apply clarsimp
-    apply (erule_tac x="<s, h>" in allE)
-    apply (erule_tac x="<s, h'>" in allE)
-    apply (erule_tac x="<a, b>" in allE)
-    using func_some func_some2 state_sep_unfold apply fastforce
-done   
-
-lemma rel_local: "safe R \<Longrightarrow> frame R \<Longrightarrow> local \<langle>R\<rangle>"
-  apply (clarsimp simp: local_def pred_leq_def)
-  apply (case_tac "\<langle>R\<rangle> (\<sigma> \<bullet> \<sigma>')") 
-  -- None apply (clarsimp simp: option.case_eq_if frame_local_Fault)
-  -- Some 
-    apply (case_tac "\<langle>R\<rangle> \<sigma> * Some {the \<sigma>'}")
-    -- None apply clarsimp
-    -- Some apply (clarsimp simp: frame_local_Some)
+  -- Some
+    apply clarsimp
+    apply (case_tac "(\<langle>R\<rangle> s (h \<bullet> h'))\<downharpoonright>\<^sup>h\<^sub>\<bottom>")
+    -- None
+      apply (clarsimp simp: safeD2_hproj)
+    -- Some
+      apply (clarsimp simp: frame_def)
+      
+      apply (meson stran2 stran3 non_faultD_hproj) 
 done
 
-lemma local_rel_safe: "local \<langle>R\<rangle> \<Longrightarrow> safe R"
-  apply (clarsimp simp: safe_def local_def state_leq_def)
-  apply (drule func_faultD)
-  by (metis (mono_tags, lifting) FaultI1 func_fault_eq option.case_eq_if pred_leq_def state_non_fault1)
-  
-lemma local_rel_frame1: "P \<subseteq> {(s, h ++ dh) |h. h \<bottom> dh \<and> (s, h) \<in> Q} \<Longrightarrow> (s, h) \<in> P \<Longrightarrow> \<exists>h'. h = h' ++ dh \<and> h' \<bottom> dh \<and> (s, h') \<in> Q"
+theorem local_safe: "local \<langle>R\<rangle> \<Longrightarrow> safe R"
+  apply (clarsimp simp: local_def safe_def substate_def stran_def)
+  apply (erule_tac x=s in allE)
+  apply (erule_tac x=h in allE)
+  apply (erule_tac x=z in allE)
+  apply clarsimp
+done
+                                                                                                                           
+lemma local_frame1: "P \<subseteq> {h \<bullet> dh |h. h ## dh \<and> h \<in> Q }\<Longrightarrow> h \<in> P \<Longrightarrow> \<exists>h'. h = h' \<bullet> dh \<and> h' ## dh \<and> h' \<in> Q"
   by auto
 
-lemma local_rel_frame2: "(<s, h>, \<sigma>') \<in> R \<Longrightarrow> \<langle>R\<rangle> <s, h> = <P> \<Longrightarrow> (<s, h>, None) \<notin> R  \<Longrightarrow> \<exists>s' h'. \<sigma>' = <s', h'> \<and> (s', h') \<in> P"
+lemma local_frame2: "(<s, h>, \<sigma>') \<in> R \<Longrightarrow> (\<langle>R\<rangle> s h)\<downharpoonright>\<^sup>h\<^sub>\<bottom> = <P> \<Longrightarrow> (<s, h>, None) \<notin> R  \<Longrightarrow> \<exists>s' h'. \<sigma>' = <s', h'> \<and> h' \<in> P"
   apply (cases \<sigma>')
   apply clarsimp
   apply (case_tac a)
-  by (simp add: func_some2)
+  by (simp add: stran3)
 
-lemma local_rel_frame: "local \<langle>R\<rangle> \<Longrightarrow> frame R"
-  apply (clarsimp simp: frame_def local_def pred_leq_def)
-  apply (erule_tac x=\<sigma>o in allE)
-  apply (erule_tac x=\<sigma>1 in allE)
+theorem local_frame: "local \<langle>R\<rangle> \<Longrightarrow> frame R"
+  apply (clarsimp simp: frame_def local_def)
+  apply (erule_tac x=so in allE)
+  apply (erule_tac x=ho in allE)
+  apply (erule_tac x=dh in allE)
   apply clarsimp
-  apply (case_tac "\<langle>R\<rangle> (\<sigma>o \<bullet> \<sigma>1)")
+  apply (case_tac "(\<langle>R\<rangle> so (ho \<bullet> dh))\<downharpoonright>\<^sup>h\<^sub>\<bottom>")
   -- None 
-    apply clarsimp
-    using FaultI1 func_fault_eq apply blast
+    using fault_eq apply fastforce
   -- Some 
     apply clarsimp
-    apply (case_tac "\<langle>R\<rangle> \<sigma>o * Some {the \<sigma>1}")
-    -- None 
-      apply clarsimp
-      using FaultI1 func_fault_eq apply blast
+    apply (case_tac "(\<langle>R\<rangle> so ho)\<downharpoonright>\<^sup>h\<^sub>\<bottom> *\<^sup>h\<^sub>\<bottom> <{dh}>")
+    -- None
+      apply (simp add: stran_def)
     -- Some
       apply clarsimp
-      apply (clarsimp simp: sep_conj_def)
-      apply (case_tac "\<langle>R\<rangle> \<sigma>o")
+      apply (case_tac "(\<langle>R\<rangle> so ho)\<downharpoonright>\<^sup>h\<^sub>\<bottom>")
       -- None
         apply clarsimp
       -- Some
-        apply (drule state_defD)
-        apply clarsimp
-        apply (rename_tac P Q s h h')
-        apply (clarsimp simp: state_sep_def )
-        apply (drule_tac local_rel_frame2)
-        apply assumption
-        apply (clarsimp simp add: func_faultD)
-        apply clarsimp
-        apply (subgoal_tac "s' = s")
-          prefer 2
-          apply blast
-        apply clarsimp
-        apply (drule local_rel_frame1)
-        apply assumption
-        apply clarsimp
-        apply (rule_tac x="Some (s, h'b)" in exI)
-        apply (auto simp add: func_some)
+        apply (clarsimp simp add: stran_hproj_eq)
+        apply (subgoal_tac "h' \<in> a")
+        apply blast
+        apply (simp add: stran3)
 done
 
-lemma local_frame_safe_eq: "local \<langle>R\<rangle> \<longleftrightarrow> safe R \<and> frame R"
-  using local_rel_frame local_rel_safe rel_local by blast
+text {* Predicate (Assertion) Level *}
 
-lemma safe_assign: "safe (assign u_upd t)"
-  apply (clarsimp simp: safe_def assign_def graph_def)
-  apply (case_tac \<sigma>)
-  --None apply clarsimp
-  -- Some
-    apply clarsimp
-    apply (case_tac \<sigma>')
-    apply auto
+definition sep :: "('a \<times> 'b) set \<Rightarrow> ('a \<times> 'b) set \<Rightarrow> ('a \<times> 'b) set" (infixl "*" 75) where
+  "P * Q \<equiv> {(s, h \<bullet> h') | s h h' .  h ## h' \<and> (s, h) \<in> P \<and> (s, h') \<in> Q}"
+
+lemma mono_star: "P \<le> Q \<Longrightarrow> P * R \<le> Q * R"
+  by (auto simp: sep_def)
+
+(* TODO: sep forms a quantale *)
+
+definition ptran :: "('a \<Rightarrow> 'b \<Rightarrow> ('a, 'b) pred_bot) \<Rightarrow> ('a \<times> 'b) set \<Rightarrow> ('a \<times> 'b) set" ("\<lbrakk>_\<rbrakk>") where
+  "\<lbrakk>f\<rbrakk> Q \<equiv> {(s, h). case f s h of \<bottom> \<Rightarrow> False | <Q'> \<Rightarrow> Q' \<subseteq> Q }"
+
+definition up_proj :: "('a, 'b) pred \<Rightarrow> ('a, 'b) pred" ("_\<up>" [1000] 999) where
+  "P\<up> \<equiv> \<top> \<times> snd ` P"
+
+definition Local :: "(('a \<times> 'b) set \<Rightarrow> ('a \<times> 'b) set) \<Rightarrow> bool" where
+  "Local F \<equiv> \<forall>P Q. (F P) * Q \<le> F (P\<up> * Q\<up>)"
+
+lemma ptranD: "(s, h) \<in> \<lbrakk>\<langle>R\<rangle>\<rbrakk> Q  \<Longrightarrow> (<s, h>, <s', h'>) \<in> R \<Longrightarrow> (s', h') \<in> Q"
+  apply (clarsimp simp: ptran_def stran_def)
+  apply (case_tac "(<s, h>, fault) \<in> R")
+  apply auto
 done
 
+lemma Local_stran_bot: "Local \<lbrakk>f\<rbrakk> \<Longrightarrow> h ## h' \<Longrightarrow> f s (h \<bullet> h') = \<bottom> \<Longrightarrow> f s h = \<bottom>"
+  apply (clarsimp simp: Local_def)
+  apply (erule_tac x="the (f s h)" in allE)
+  apply (erule_tac x="{(s, h')}" in allE)
+  apply (case_tac "f s h")
+  apply (clarsimp simp: ptran_def)
+  apply (subgoal_tac "the (f s h) = a")
+  apply (force simp: ptran_def sep_def)
+  apply force
+done
 
-
-lemma "frame (assign u_upd t)"
-  apply (auto simp: frame_def)
-  apply (frule state_defD)
+lemma Local_stran_bot2: "Local \<lbrakk>\<langle>R\<rangle>\<rbrakk> \<Longrightarrow> h ## h' \<Longrightarrow> (\<langle>R\<rangle> s (h \<bullet> h'))\<downharpoonright>\<^sup>h\<^sub>\<bottom> = \<bottom> \<Longrightarrow> (\<langle>R\<rangle> s h)\<downharpoonright>\<^sup>h\<^sub>\<bottom> = \<bottom>"
+  apply (clarsimp simp: stran_def sep_def ptran_def Local_def)
+  apply (erule_tac x="{\<sigma>'. (<s, h>, <\<sigma>'>) \<in> R}" in allE)
+  apply (erule_tac x="{(s, h')}" in allE)
   apply clarsimp
-  apply (case_tac \<sigma>')
+  apply (case_tac " (<s, h \<bullet> h'>, fault) \<in> R")
+  apply force
+  apply clarsimp
+done
+
+lemma stran_ptran: "f s h = <S> \<Longrightarrow> (s, h) \<in> \<lbrakk>f\<rbrakk> S"
+  by (clarsimp simp: stran_def ptran_def)
+
+lemma stran_ptran_eq2: "f s h = <S> \<Longrightarrow> S \<subseteq> S' \<longleftrightarrow> (s, h) \<in> \<lbrakk>f\<rbrakk> S'"
+  apply (clarsimp simp: stran_def ptran_def)
+done
+
+lemma stran_ptran_eq: "(f s h)\<downharpoonright>\<^sup>h\<^sub>\<bottom> \<subseteq>\<^sup>h\<^sub>\<bottom> <H> \<longleftrightarrow> (s, h) \<in> \<lbrakk>f\<rbrakk> (\<top>\<times>H)"
+  apply (clarsimp simp: stran_def ptran_def)
+  apply (case_tac "f s h")
+  apply auto
+done
+
+lemma stran_ptranD [dest]: "(f s h)\<downharpoonright>\<^sup>h\<^sub>\<bottom> = <H> \<Longrightarrow> (s, h) \<in> \<lbrakk>f\<rbrakk> (\<top>\<times>H)"
+  using stran_ptran_eq by force
+
+lemma sep_heap_only[simp]: "\<top>\<times>H * \<top>\<times>H' = \<top>\<times>{h \<bullet> h' |h h'. h ## h' \<and> h \<in> H \<and> h' \<in> H'}"
+  by (auto simp: sep_def)
+
+theorem Local_local: "Local \<lbrakk>f\<rbrakk> \<Longrightarrow> local f"
+  apply (clarsimp simp: local_def up_proj_def)
+  apply (case_tac "(f s h)\<downharpoonright>\<^sup>h\<^sub>\<bottom> *\<^sup>h\<^sub>\<bottom> <{h'}>")
+  -- None 
+    apply clarsimp
+  -- Some 
+    apply (clarsimp simp: stran_ptran_eq)
+    apply (case_tac "(f s h)\<downharpoonright>\<^sup>h\<^sub>\<bottom>")
+    -- None
+    apply clarsimp
+    -- Some
+    apply (clarsimp simp: Local_def up_proj_def)
+    apply (erule_tac x="\<top>\<times>aa" in allE)
+    apply (erule_tac x="\<top>\<times>{h'}" in allE) 
+    using sep_def apply fastforce
+done
+
+
+lemma local_Local_bot: "local f \<Longrightarrow> (a, b) \<in> \<lbrakk>f\<rbrakk> P * Q \<Longrightarrow> f a b = \<bottom> \<Longrightarrow> (a, b) \<in> \<lbrakk>f\<rbrakk> (\<top> \<times> {h \<bullet> h' |h h'. h ## h' \<and> h \<in> P\<downharpoonright>\<^sup>h \<and> h' \<in> Q\<downharpoonright>\<^sup>h})"
+  apply (clarsimp simp: ptran_def sep_def local_def)
+  apply (erule_tac x=a in allE)
+  apply (erule_tac x=h in allE)
+  apply (erule_tac x=h' in allE)
+  apply clarsimp
+  apply (case_tac "f a h")
+  apply auto
+done
+
+theorem local_Local: "local f  \<Longrightarrow> Local \<lbrakk>f\<rbrakk>"
+  apply (clarsimp simp: Local_def)
+  apply (case_tac "f a b")
   -- None
-    apply (clarsimp simp add: safe_assign safe_fault)
+    apply (simp add: local_Local_bot up_proj_def)
   -- Some
+    apply (rename_tac P')
+    apply (subst stran_ptran_eq2[symmetric])
+    apply assumption
+    apply (default, case_tac x, clarsimp)
+    apply (clarsimp simp: local_def)
+    apply (rename_tac s h F s' h')
+    apply (subgoal_tac "\<exists>h1 h2 F1. h = h1 \<bullet> h2 \<and> h1 ## h2 \<and> f s h1 = <F1> \<and> F1 \<subseteq> P \<and> h2 \<in> snd ` Q")
+      apply clarsimp
+      apply (erule_tac x=s in allE)
+      apply (erule_tac x=h1 in allE)
+      apply (erule_tac x=b in allE)
+      apply clarsimp
+      apply (subgoal_tac "h' \<in> {y. \<exists>x\<in>F. y = snd x}")
+        apply (subgoal_tac "h' \<in> {h \<bullet> b |h. h ## b \<and> (\<exists>x\<in>F1. h = snd x)}")
+        apply (clarsimp simp: up_proj_def)
+        apply (rule_tac x=bb in exI)
+        apply (rule_tac x=b in exI)
+        apply (force simp: sep_def)
+        apply force
+      apply force
+    apply (clarsimp simp: sep_def)
+    apply (rule_tac x=ha in exI)
+    apply (rule_tac x=h'a in exI)
     apply clarsimp
-    apply (clarsimp simp: assign_def graph_def)
-    apply (case_tac "<s, h> \<bullet> <s, h'>")
-    apply clarsimp
-    apply clarsimp
+    apply (case_tac "f s ha")
+    -- None 
+      apply (clarsimp simp add: ptran_def)
+    -- Some
+    apply (subst (asm) stran_ptran_eq2[symmetric])
+    apply assumption
+    apply force
+done
 
+definition about_heap :: "('a \<times> 'b) set \<Rightarrow> bool" where
+  "about_heap P \<equiv> P = P\<up>"
 
+lemma frame_rule: "Local F \<Longrightarrow> about_heap Q \<Longrightarrow> about_heap R \<Longrightarrow> P \<le> F Q \<Longrightarrow> P * R \<le> F (Q * R)"
+  apply (simp add: about_heap_def Local_def)
+  by (metis dual_order.trans mono_star)
 
-
-
-
-
-
+end
 
 end
