Algebra/PartialMonoid.thy
@@ -1,0 +1,222 @@
+theory PartialMonoid
+  imports Main
+begin
+
+section {* Partial monoid *}
+
+no_notation 
+  one_class.one ("1") and
+  times (infixl "*" 70)
+
+notation bot ("\<bottom>")
+
+text {* Signature of our classes *}
+
+class pmult =
+  fixes pmult :: "'a \<Rightarrow> 'a \<Rightarrow> 'a" (infixl "\<oplus>" 80)
+
+class pmult_defined =
+  fixes pmult_defined :: "'a \<Rightarrow> 'a \<Rightarrow> bool" (infix "##" 55)
+
+class pmult_one =
+  fixes pmult_one :: "'a" ("1")
+
+text {* Domain theoretical way of defining pmult semigroups, i.e., adding a \<bottom> (seeking) element. *}
+
+class partial_semigroup_bot = pmult + bot +
+  assumes pbot_assoc: "(x \<oplus> y) \<oplus> z = x \<oplus> (y \<oplus> z)"
+  and botl [simp]: "x \<oplus> \<bottom> = \<bottom>"
+  and botr [simp]: "\<bottom> \<oplus> x = \<bottom>"
+
+text {* 
+  Let the binary relation ## be: x ## y \<longleftrightarrow> x + y \<noteq> \<bottom>, one can naturally define the
+  following class based on the pmult semigroup with bottom element.
+*}
+
+class partial_semigroup_var = pmult + pmult_defined +
+  assumes pmult_defr: "x ## (y \<oplus> z) \<Longrightarrow> y ## z"
+  and pmult_defl: "(x \<oplus> y) ## z \<Longrightarrow> x ## y"
+  and pmult_def_assoc: "x ## (y \<oplus> z) = (x \<oplus> y) ## z"
+  and pmult_assoc_var: "x ## (y \<oplus> z) \<Longrightarrow> (x \<oplus> y) \<oplus> z = x \<oplus> (y \<oplus> z)"
+
+text {*
+  A simpler pmult semigroup can be defined where it states that if x * y and (x * y) * z 
+  are defined, then y * z is also defined.
+*}
+
+class partial_semigroup = pmult + pmult_defined +
+  assumes pmult_def: "(x \<oplus> y) ## z \<and> x ## y \<longleftrightarrow> x ## (y \<oplus> z) \<and> y ## z"
+  and pmult_assoc: "\<lbrakk>x ## (y \<oplus> z); x ## y\<rbrakk> \<Longrightarrow> (x \<oplus> y) \<oplus> z = x \<oplus> (y \<oplus> z)"
+
+class totality = pmult_defined +
+  assumes totality[simp]: "x ## y"
+
+class total_semigroup = partial_semigroup + totality
+begin
+
+lemma total_assoc: "(x \<oplus> y) \<oplus> z = x \<oplus> (y \<oplus> z)"
+  by (metis pmult_assoc totality)
+
+sublocale semigroup "op \<oplus>" 
+  by default (simp add: total_assoc)
+
+end
+
+text {* 
+  As expected, the pmult semigroup with bottom element is the strongest, where one can
+  derive the other classes.
+*}
+
+sublocale partial_semigroup_bot \<subseteq> partial_semigroup_var "op \<oplus>" "\<lambda>x y. x \<oplus> y \<noteq> \<bottom>"
+  by (default, metis botl, metis botr, (metis pbot_assoc)+)
+
+sublocale partial_semigroup_var \<subseteq> partial_semigroup
+  by default (metis pmult_def_assoc pmult_defl pmult_defr, metis pmult_assoc_var)
+
+sublocale partial_semigroup_bot \<subseteq> partial_semigroup "op \<oplus>" "\<lambda>x y. x \<oplus> y \<noteq> \<bottom>" ..
+
+text {*
+  We select the weakest pmult semigroup to continue our hierarchy up to commutative monoid.
+*}
+
+class partial_ab_semigroup = pmult + pmult_defined +
+  assumes pmult_ab_def: "(x \<oplus> y) ## z \<and> x ## y \<Longrightarrow> x ## (y \<oplus> z) \<and> y ## z"
+  and pmult_ab_assoc: "\<lbrakk>x ## (y \<oplus> z); x ## y\<rbrakk> \<Longrightarrow> (x \<oplus> y) \<oplus> z = x \<oplus> (y \<oplus> z)"
+  and pmult_comm_def: "x ## y \<Longrightarrow> y ## x"
+  and pmult_comm: "x ## y \<Longrightarrow> x \<oplus> y = y \<oplus> x"
+begin
+
+lemma pmult_ab1: "(x \<oplus> y) ## z \<Longrightarrow> x ## y \<Longrightarrow> x ## (y \<oplus> z)"
+  by (metis pmult_ab_def)
+
+lemma pmult_ab2: "(x \<oplus> y) ## z \<and> x ## y \<Longrightarrow> y ## z"
+  by (metis pmult_ab_def)
+
+lemma "x ## y = y ## x"
+  by (metis pmult_comm_def)
+
+lemma pmult_def_eq: "(x \<oplus> y) ## z \<and> x ## y \<longleftrightarrow> x ## (y \<oplus> z) \<and> y ## z"
+  by (metis pmult_comm_def pmult_ab_def)
+
+lemma pmult_ab3: "x ## (y \<oplus> z) \<Longrightarrow> y ## z \<Longrightarrow> (x \<oplus> y) ## z"
+  by (metis pmult_def_eq)
+
+lemma pmult_ab4: "x ## (y \<oplus> z) \<Longrightarrow> y ## z \<Longrightarrow> x ## y"
+  by (metis pmult_def_eq)
+
+subclass partial_semigroup 
+  by default (metis pmult_def_eq, metis pmult_ab_assoc)
+
+end
+
+class total_ab_semigroup = partial_ab_semigroup + totality
+begin
+
+lemma total_assoc: "(x \<oplus> y) \<oplus> z = x \<oplus> (y \<oplus> z)"
+  by (metis pmult_assoc totality)
+
+lemma total_comm: "x \<oplus> y = y \<oplus> x"
+  by (metis pmult_comm totality)
+
+subclass total_semigroup ..
+
+end
+                                     
+class partial_monoid = partial_semigroup + pmult_one + 
+  assumes pmult_one_defr [simp]: "x ## 1"
+  and pmult_one_defl [simp]: "1 ## x"
+  and pmult_oner: "x \<oplus> 1 = x"
+  and pmult_onel: "1 \<oplus> x = x"
+
+class total_monoid = partial_monoid + totality
+begin
+subclass total_semigroup ..
+
+sublocale monoid "op \<oplus>" 1
+  by default (simp_all add: pmult_oner pmult_onel)
+
+end
+
+class partial_comm_monoid = partial_ab_semigroup + pmult_one +
+  assumes pone_defr: "x ## 1"
+  and poner: "x \<oplus> 1 = x"
+begin
+
+subclass partial_monoid
+  by default (auto simp: pone_defr poner pmult_comm pmult_comm_def)
+
+end
+
+class total_comm_monoid = partial_comm_monoid + totality
+begin
+subclass total_ab_semigroup ..
+subclass total_monoid ..
+
+sublocale comm_monoid "op \<oplus>" 1
+  by default (simp_all add: total_comm)
+end
+
+section {* Models of partial monoids *}
+
+text {* 
+  The natural model of a partial monoid is partial functions. 
+*}
+
+typedef ('a, 'b) pfun = "UNIV :: ('a \<Rightarrow> 'b option) set" ..
+setup_lifting type_definition_pfun
+
+instantiation pfun :: (type, type) partial_semigroup
+begin
+lift_definition pmult_pfun :: "('a, 'b) pfun \<Rightarrow> ('a, 'b) pfun \<Rightarrow> ('a, 'b) pfun" is map_add .
+lift_definition pmult_defined_pfun :: "('a, 'b) pfun \<Rightarrow> ('a, 'b) pfun \<Rightarrow> bool" is "\<lambda>x y. dom x \<inter> dom y = {}" .
+instance 
+  by default (transfer, fastforce)+
+end
+
+instantiation pfun :: (type, type) partial_monoid
+begin
+lift_definition pmult_one_pfun :: "('a, 'b) pfun" is empty .
+instance
+  by default (transfer, fastforce)+
+end
+
+text {*
+  We can also have a model where we add a new bottom element.
+*}
+
+typedef ('a, 'b) pfun_bot = "UNIV :: ('a \<Rightarrow> ('b option) option) set" ..
+setup_lifting type_definition_pfun_bot
+
+instantiation pfun_bot :: (type, type) partial_semigroup_bot
+begin
+lift_definition bot_pfun_bot :: "('a, 'b) pfun_bot" is "\<lambda>x. Some None" .
+lift_definition pmult_pfun_bot :: "('a, 'b) pfun_bot \<Rightarrow> ('a, 'b) pfun_bot \<Rightarrow> ('a, 'b) pfun_bot" 
+  is "\<lambda>x y. if dom x \<inter> dom y = {} then map_add x y else (\<lambda>x. Some None)" .
+
+instance
+  by default (transfer, fastforce)+
+end
+
+text {*
+  And obviously, it is also a model for our weaker semigroup.
+*}
+
+instantiation pfun_bot :: (type, type) partial_semigroup
+begin
+lift_definition pmult_defined_pfun_bot :: "('a, 'b) pfun_bot \<Rightarrow> ('a, 'b) pfun_bot \<Rightarrow> bool" is
+  "\<lambda>x y. dom x \<inter> dom y = {}" .
+instance
+  by default (transfer, auto)+
+end
+
+text {*
+  We could instantiate the heap as a partial function from nat to nat
+*}
+(*type_synonym heap = "(nat, nat) pfun"*)
+
+notation one_class.one ("1")
+
+no_notation bot ("\<bottom>")
+
+
+end
