Snippets/Thesis.thy
@@ -1,0 +1,5 @@
+theory Thesis
+  imports Chapter1
+begin
+
+end
